Fp/Theorems/UnpackedRound.lean
@@ -6,12 +6,14 @@ import Fp.Theorems.Packing
 
 
 namespace Fp
+open SmtLibSemantics
 
 @[simp]
 theorem roundQ_eq (eout sout : Nat) (rm : RoundingMode) (sign : Bool) (r : ExtRat):
     (Fp.SmtLibSemanticsQ.smtLibRoundMethodQ eout sout).round rm sign r =
     (SmtLibSemantics.smtLibRoundMethod eout sout
-      SmtLibSemantics.smtLibV SmtLibSemantics.smtLibV).round rm sign
+      (SmtLibSemantics.smtLibV (SmtLibSemantics.embedPackedFloatExtRat eout sout))
+      (SmtLibSemantics.smtLibV (SmtLibSemantics.embedPackedFloatExtRat eout (sout + 1)))).round rm sign
     r := rfl
 
 set_option warn.sorry false in
@@ -26,32 +28,42 @@ theorem upper_NaN_eq_PackedFloat_mkNaN :
 
 @[simp]
 theorem roundRNA_mkNaN (eout sout : Nat) (sign : Bool) :
-  (SmtLibSemantics.smtLibRoundMethod eout sout SmtLibSemantics.smtLibV SmtLibSemantics.smtLibV).roundRNA sign
+  (SmtLibSemantics.smtLibRoundMethod eout sout
+    (SmtLibSemantics.smtLibV (SmtLibSemantics.embedPackedFloatExtRat eout sout))
+    (SmtLibSemantics.smtLibV (SmtLibSemantics.embedPackedFloatExtRat eout (sout + 1)))).roundRNA sign
     (ExtRat.NaN) = PackedFloat.mkNaN := by
   simp [SmtLibSemantics.RoundMethod.roundRNA]
 
 @[simp]
 theorem roundRNE_mkNaN (eout sout : Nat) (sign : Bool) :
-  (SmtLibSemantics.smtLibRoundMethod eout sout SmtLibSemantics.smtLibV SmtLibSemantics.smtLibV).roundRNE sign
+  (SmtLibSemantics.smtLibRoundMethod eout sout
+    (SmtLibSemantics.smtLibV (SmtLibSemantics.embedPackedFloatExtRat eout sout))
+    (SmtLibSemantics.smtLibV (SmtLibSemantics.embedPackedFloatExtRat eout (sout + 1)))).roundRNE sign
     (ExtRat.NaN) = PackedFloat.mkNaN := by
   simp [SmtLibSemantics.RoundMethod.roundRNE]
 
 @[simp]
 theorem roundRTP_mkNaN (eout sout : Nat) (sign : Bool) :
-  (SmtLibSemantics.smtLibRoundMethod eout sout SmtLibSemantics.smtLibV SmtLibSemantics.smtLibV).roundRTP sign
+  (SmtLibSemantics.smtLibRoundMethod eout sout
+    (SmtLibSemantics.smtLibV (SmtLibSemantics.embedPackedFloatExtRat eout sout))
+    (SmtLibSemantics.smtLibV (SmtLibSemantics.embedPackedFloatExtRat eout (sout + 1)))).roundRTP sign
     (ExtRat.NaN) = PackedFloat.mkNaN := by
   simp [SmtLibSemantics.RoundMethod.roundRTP]
 
 @[simp]
 theorem roundRTN_mkNaN (eout sout : Nat) (sign : Bool) :
-  (SmtLibSemantics.smtLibRoundMethod eout sout SmtLibSemantics.smtLibV SmtLibSemantics.smtLibV).roundRTN sign
+  (SmtLibSemantics.smtLibRoundMethod eout sout
+    (SmtLibSemantics.smtLibV (SmtLibSemantics.embedPackedFloatExtRat eout sout))
+    (SmtLibSemantics.smtLibV (SmtLibSemantics.embedPackedFloatExtRat eout (sout + 1)))).roundRTN sign
     (ExtRat.NaN) = PackedFloat.mkNaN := by
   simp [SmtLibSemantics.RoundMethod.roundRTN]
   rcases sign <;> simp
 
 @[simp]
 theorem rountRTZ_mkNaN (eout sout : Nat) (sign : Bool) :
-  (SmtLibSemantics.smtLibRoundMethod eout sout SmtLibSemantics.smtLibV SmtLibSemantics.smtLibV).roundRTZ sign
+  (SmtLibSemantics.smtLibRoundMethod eout sout
+    (SmtLibSemantics.smtLibV (SmtLibSemantics.embedPackedFloatExtRat eout sout))
+    (SmtLibSemantics.smtLibV (SmtLibSemantics.embedPackedFloatExtRat eout (sout + 1)))).roundRTZ sign
     (ExtRat.NaN) = PackedFloat.mkNaN := by
   simp [SmtLibSemantics.RoundMethod.roundRTZ]
   rcases sign <;> simp
@@ -59,7 +71,9 @@ theorem rountRTZ_mkNaN (eout sout : Nat) (sign : Bool) :
 
 @[simp]
 theorem round_eq_mkNaN_of_NaN {sign} {eout sout : Nat} {rm : RoundingMode} :
-    (SmtLibSemantics.smtLibRoundMethod eout sout SmtLibSemantics.smtLibV SmtLibSemantics.smtLibV).round
+    (SmtLibSemantics.smtLibRoundMethod eout sout
+      (SmtLibSemantics.smtLibV (SmtLibSemantics.embedPackedFloatExtRat eout sout))
+      (SmtLibSemantics.smtLibV (SmtLibSemantics.embedPackedFloatExtRat eout (sout + 1)))).round
         rm sign ExtRat.NaN = PackedFloat.mkNaN := by
   rcases rm
   · simp
@@ -71,7 +85,10 @@ theorem round_eq_mkNaN_of_NaN {sign} {eout sout : Nat} {rm : RoundingMode} :
 set_option warn.sorry false in
 @[simp]
 theorem round_eq_mkZero_of_mkZero {zeroSign : Bool} {eout sout : Nat} {rm : RoundingMode} :
-    (SmtLibSemantics.smtLibRoundMethod eout sout SmtLibSemantics.smtLibV SmtLibSemantics.smtLibV).round
+    (SmtLibSemantics.smtLibRoundMethod eout sout
+      (SmtLibSemantics.smtLibV (SmtLibSemantics.embedPackedFloatExtRat eout sout))
+      (SmtLibSemantics.smtLibV (SmtLibSemantics.embedPackedFloatExtRat eout (sout + 1)))
+    ).round
         rm zeroSign (ExtRat.Number 0) = PackedFloat.getZero eout sout zeroSign := by
   rcases rm <;> sorry
 
@@ -80,11 +97,11 @@ theorem round_eq_mkZero_of_mkZero {zeroSign : Bool} {eout sout : Nat} {rm : Roun
 -/
 structure ApproximatesUptoRounding (uf : UnpackedFloat ein sin) (er : ExtRat) (eout sout : Nat) : Prop where
   /-- we have at least 2 bits more, of guard and sticky. -/
-  hSigGe : sin + 2 ≥ sout 
+  hSigGe : sin + 2 ≥ sout
   /-- we have at least as much exponent range. -/
   hExpGe : ein ≥ eout -- we have at least as much exponent range
   /-- rational values have (sout + 1) bits of precision. -/
-  hApproxUptoGuard : ∀ (r : Rat), .Number r = er → (uf.toRat - r).abs < (2 : Rat) ^ (-(sout + 1 : Int)) 
+  hApproxUptoGuard : ∀ (r : Rat), .Number r = er → (uf.toRat - r).abs < (2 : Rat) ^ (-(sout + 1 : Int))
   /-- the sticky bit is zero iff the number truncated upto the guard bit equals -/
   hStickyBitCorrect : ∀ (r : Rat), .Number r = er → ((uf.sig.extractMsb' (sout + 1) (sin - (sout + 1)) ≠ 0) = decide (r = uf.toRat))
 
@@ -92,7 +109,10 @@ set_option warn.sorry false in
 theorem roundQ_Number_eq_round
     (er : ExtRat) (uf : UnpackedFloat ein sin)
     (hruf : ApproximatesUptoRounding uf er eout sout) (rm : RoundingMode) (sign : Bool) :
-    (SmtLibSemantics.smtLibRoundMethod eout sout SmtLibSemantics.smtLibV SmtLibSemantics.smtLibV).round rm sign
+    (SmtLibSemantics.smtLibRoundMethod eout sout
+      (SmtLibSemantics.smtLibV (SmtLibSemantics.embedPackedFloatExtRat eout sout))
+      (SmtLibSemantics.smtLibV (SmtLibSemantics.embedPackedFloatExtRat eout (sout + 1)))
+    ).round rm sign
       er =
       (UnpackedFloat.round uf rm).pack := by sorry
 
@@ -111,42 +131,20 @@ theorem roundQ_Number_eq_round
 
 @[simp]
 theorem roundQ_eq_round_of_Infinity {zeroSign infSign : Bool} {e s : Nat} {rm : RoundingMode} :
-    (SmtLibSemantics.smtLibRoundMethod e s SmtLibSemantics.smtLibV SmtLibSemantics.smtLibV).round rm zeroSign
+    (SmtLibSemantics.smtLibRoundMethod e s
+      (SmtLibSemantics.smtLibV (SmtLibSemantics.embedPackedFloatExtRat e s))
+      (SmtLibSemantics.smtLibV (SmtLibSemantics.embedPackedFloatExtRat e (s + 1)))
+    ).round rm zeroSign
       (ExtRat.Infinity infSign) =
       PackedFloat.getInfinity e s infSign := by sorry
 
-/--
-Case splitting on the different values a packed float
-can have: it can be nan, infinity, zero, or a nonzero normal/subnormal.+
--/
-@[elab_as_elim]
-theorem PackedFloat.kindCasesNaNInfZeroNum {P : PackedFloat e s → Prop}
-    (x : PackedFloat e s)
-    (nanCase : ∀ (n : PackedFloat e s), n.isNaN → P n)
-    (infCase : ∀ sign, P (PackedFloat.getInfinity e s sign))
-    (zeroCase : ∀ sign, P (PackedFloat.getZero e s sign))
-    (numCase : ∀ (n : PackedFloat e s), n.isNormOrNonzeroSubnorm → P n) :
-    P x := by
-  have := x.classification_exhaustive
-  simp at this
-  by_cases h1 : x.isNaN
-  · grind
-  · by_cases h2 : x.isInfinite
-    · grind
-    · by_cases h3 : x.isZero
-      · grind
-      · by_cases h4 : x.isNonzeroSubnorm
-        · grind
-        · by_cases h5 : x.isNorm
-          · grind
-          · grind
 
 @[grind <=]
 theorem PackedFloat.eq_of_unpack_eq_unpack_of_isInfinity {x y : PackedFloat e s}
     (hs : 0 < s) (he : 0 < e)
     (hx : x.isInfinite) (hy : y.isInfinite) (h : x.unpack = y.unpack) :
     x = y := by
-  cases x using PackedFloat.kindCasesNaNInfZeroNum <;> try grind
+  cases x using PackedFloat.classification <;> try grind
 
 /--
 Purely arithmetic fact that needs to be proven,
@@ -173,7 +171,7 @@ theorem mul_eq_mul {ein sin : Nat} (hsin : 0 < sin) (he : 0 < ein)
     rm a b = PackedFloat.mul rm a b := by
   simp [SmtLibSemantics.SmtLibFunctions.mul]
   rw [PackedFloat.mul, EUnpackedFloat.mul]
-  cases a using PackedFloat.kindCasesNaNInfZeroNum
+  cases a using PackedFloat.classification
   case nanCase hnan =>
     simp [hnan]
     rw [round_eq_mkNaN_of_NaN]
@@ -182,7 +180,7 @@ theorem mul_eq_mul {ein sin : Nat} (hsin : 0 < sin) (he : 0 < ein)
     rw [← ExtRat.mul_def]
     unfold ExtRat.mul
     simp
-    cases b using PackedFloat.kindCasesNaNInfZeroNum
+    cases b using PackedFloat.classification
     case nanCase hb =>
       simp [hb]
       -- | why does this not apply automatically?
@@ -213,7 +211,7 @@ theorem mul_eq_mul {ein sin : Nat} (hsin : 0 < sin) (he : 0 < ein)
       sorry
   case zeroCase sign =>
     simp [he]
-    cases b using PackedFloat.kindCasesNaNInfZeroNum
+    cases b using PackedFloat.classification
     case nanCase hb =>
       simp [hb]
       rw [round_eq_mkNaN_of_NaN]
@@ -240,7 +238,7 @@ theorem mul_eq_mul {ein sin : Nat} (hsin : 0 < sin) (he : 0 < ein)
     rw [PackedFloat.unpack_eq_mkNumber_of_isNormOrNonzeroSubnorm ha]
     rw [PackedFloat.toExtRat'_eq_Number_of_isNormOrNonzeroSubnorm ha]
     -- interesting case, when a is a number.
-    cases b using PackedFloat.kindCasesNaNInfZeroNum
+    cases b using PackedFloat.classification
     case nanCase hb =>
       simp [hb]
       rw [round_eq_mkNaN_of_NaN]
